Juvix/Core/Main/Language/Value.lean
@@ -4,10 +4,10 @@ import Juvix.Core.Main.Language.Base
 namespace Juvix.Core.Main
 
 inductive Value : Type where
+  | unit : Value
   | const : Constant → Value
   | constr_app : (constr : Name) → (args_rev : List Value) → Value
   | closure : (ctx : List Value) → (value : Expr) → Value
-  | unit : Value
   deriving Inhabited
 
 abbrev Context : Type := List Value
