Juvix/Utils.lean
@@ -1,0 +1,40 @@
+
+import Aesop
+
+namespace Juvix.Utils
+
+theorem monotone_ex_all {α} {P : Nat → α → Prop}
+  (mh: ∀ n n' x, P n x → n ≤ n' → P n' x)
+  (l : List α)
+  (h : ∀ x ∈ l, ∃ n, P n x) : ∃ n, ∀ x ∈ l, P n x := by
+  induction l with
+  | nil =>
+    exists 0
+    aesop
+  | cons x xs ih =>
+    obtain ⟨n, hn⟩ := h x (by simp)
+    obtain ⟨m, hm⟩ := ih (λ x hx => h x (by simp [hx]))
+    exists (Max.max n m)
+    intros x' hx'
+    cases hx'
+    case intro.head =>
+      apply mh
+      exact hn
+      exact Nat.le_max_left n m
+    case intro.tail ht =>
+      apply (mh m (Max.max n m) x')
+      aesop
+      exact Nat.le_max_right n m
+
+theorem zip_refl_eq {α} (l : List α) (p : α × α) (h : p ∈ List.zip l l) : p.fst = p.snd := by
+  induction l with
+  | nil =>
+    cases h
+  | cons x xs ih =>
+    cases h
+    case cons.head =>
+      simp
+    case cons.tail ht =>
+      exact ih ht
+
+end Juvix.Utils
